proof/correctness/Correctness_Mem.ec
@@ -1,0 +1,59 @@
+pragma Goals : printall.
+
+require import AllCore List RealExp IntDiv.
+
+from Jasmin require import JModel.
+
+require import Array128 Array4.
+require import XMSS_IMPL.
+
+require import Array128 Array4.
+require import XMSS_IMPL.
+
+lemma memset_4_post (input : W8.t Array4.t, v : W8.t) :
+    hoare [M(Syscall).__memset_u8_4 : arg=(input, v) ==> 
+     (forall (k : int), 0 <= k < 4 => (res.[k] = v))].
+proof.
+proc.
+while (
+  0 <= to_uint i <= 4 /\ 
+  value = v /\
+  (forall (k : int), 0 <= k < to_uint i => (a.[k] = value))
+); auto => /> *.
+- do split.
+  + smt(@W64).
+  + smt(@W64).
+  + move => ???. rewrite get_setE ; smt(@W64).
+- progress ; [ smt(@W64) | smt ].
+qed.
+
+lemma memset_128_post (input : W8.t Array128.t, v : W8.t) :
+    hoare [M(Syscall).__memset_u8_128 : arg=(input, v) ==> 
+     (forall (k : int), 0 <= k < 128 => (res.[k] = v))].
+proof.
+proc.
+while (
+  0 <= to_uint i <= 128 /\ 
+  value = v /\
+  (forall (k : int), 0 <= k < to_uint i => (a.[k] = value))
+); auto => /> *.
+- do split.
+  + smt(@W64).
+  + smt(@W64).
+  + move => ???. rewrite get_setE ; smt(@W64).
+- progress ; [ smt(@W64) | smt ].
+qed.
+
+lemma memset_4_ll : islossless M(Syscall).__memset_u8_4.
+proof.
+proc.
+while (0 <= to_uint i <= 4) (4 - (to_uint i)) ; auto => /> * ; last by smt(@W64).
+do split; 1,3: by rewrite to_uintD_small /#. smt(@W64).
+qed.
+
+lemma memset_128_ll : islossless M(Syscall).__memset_u8_128.
+proof.
+proc.
+while (0 <= to_uint i <= 128) (128 - (to_uint i)) ; auto => /> * ; last by smt(@W64).
+do split; 1,3: by rewrite to_uintD_small /#. smt(@W64).
+qed.
