proof/correctness/Correctness_Wots.ec
@@ -8,393 +8,69 @@ require import XMSS_IMPL XMSS_IMPL_PP Generic.
 
 require import Array2 Array3 Array8 Array32 Array67 Array2144.
 
-(*****************************************************************************************************************)
-
-lemma take_drop_3 (x : 'a Array3.t) (v : 'a) (i : int) :
-    take i (mkseq ("_.[_]" x) 3) ++ v :: drop (i + 1) (mkseq ("_.[_]" x) 3) =
-    mkseq ("_.[_]" x.[i <- v]) 3.
+lemma nosmt shr_ge0 (input : W8.t Array32.t) (i : W64.t) :
+    0 <= to_uint i < 32 =>
+    0 <= to_uint ((SHR_32 (zeroextu32 input.[to_uint i]) (truncateu8 ((of_int 4))%W64)).`6 `&` (of_int 15)%W32).
 proof.
-case (0 <= i /\ i < 3).
-move => H. move : H => [#] i_ge0 i_lt3.
-pose s := mkseq ("_.[_]" x) 3.
-rewrite -put_in.
-smt(size_mkseq).
-admit.
-move => H.
+move => [i_ge0 i_lt_32].
 admit.
 qed.
 
-
-lemma array3_list_put ['a] (x : 'a Array3.t) (v : 'a) (i : int) : put (to_list x) i v = to_list (x.[i <- v]).
+lemma nosmt shr_lt_15 (input : W8.t Array32.t) (i : W64.t) :
+    0 <= to_uint i < 32 =>
+    to_uint ((SHR_32 (zeroextu32 input.[to_uint i]) (truncateu8 ((of_int 4))%W64)).`6 `&` (of_int 15)%W32) <= 15.
 proof.
-rewrite /to_list /put => />.
-case (0 <= i /\ i < 3).
-move => H.
-move : H => [#] i_ge0 i_lt3.
-rewrite ifT.
-split ; first by apply i_ge0. 
-smt(@List).
-apply take_drop_3.
-move => H.
-rewrite ifF.
-smt(@List).
-congr.
-smt(@Array3).
-qed.
-
-
-lemma take_drop_67 (x : 'a Array67.t) (v : 'a) (i : int) :
-    take i (mkseq ("_.[_]" x) 67) ++ v :: drop (i + 1) (mkseq ("_.[_]" x) 67) =
-    mkseq ("_.[_]" x.[i <- v]) 67.
-proof.
-case (0 <= i /\ i < 67).
-move => H. 
-move : H => [#] i_ge0 i_lt67.
-pose s := mkseq ("_.[_]" x) 67.
-rewrite -put_in.
-smt(size_mkseq).
-admit.
+move => [i_ge0 i_lt_32].
 admit.
 qed.
 
 
-lemma array67_list_put ['a] (x : 'a Array67.t) (v : 'a) (i : int) : put (to_list x) i v = to_list (x.[i <- v]).
-proof.
-rewrite /to_list /put => />.
-case (0 <= i /\ i < 67).
-move => H. 
-move : H => [#] i_ge0 i_lt67.
-rewrite ifT.
-split ; first by apply i_ge0.
-smt(@List).
-apply take_drop_67.
-move => H.
-rewrite ifF.
-smt(@List).
-congr.
-smt(@Array67).
-qed.
-
-(*****************************************************************************************************************)
-
-lemma foo (i y : W64.t) :
- ! (i \ult y) = y \ule i by smt.
-
-lemma plus_one (x : W64.t) :
-(*     to_uint x < W64.max_uint =>  *)
-    to_uint x + 1 = to_uint (x + W64.one).
-proof.
-admit.
-qed.
-
-
-lemma lt (x y : W64.t) :
-    x \ult y => x + W64.one \ule y by smt.
-
-
-(*****************************************************************************************************************)
-
-
-lemma f0 (x y : W64.t) : to_uint (x - y) <= 0 <=> ! (y \ult x) by smt.
-lemma f1 (x y : int) : x - y <= 0 <=> ! (y < x) by smt().
-lemma f2 (x y : W64.t) :
-    to_uint (x - (y + W64.one)) < to_uint (x - y) by smt.
-
-(*****************************************************************************************************************)
-
-
-(* 
-base w 
-TERMINATION : DONE 
-CORRECTNESS : Auxiliary lemmas with admit
-*)
-lemma base_w_ll : islossless BaseWGeneric.__base_w.
+lemma nosmt base_w_67_post :
+    hoare [M(Syscall).__base_w_67_32 : true ==>
+      forall (k : int), 0 <= k < 67 => (0 <= to_uint res.[k] <= 15)]. (* 15 = w - 1 *)
 proof.
 proc.
-islossless.
-while (true) ((to_uint outlen) - (to_uint consumed)) ; first by auto => /> *; smt(@W64).
-skip.
-auto => /> /#.
+while (
+  0 <= to_uint i <= 67 /\
+  0 <= to_uint total <= 15 /\
+  (forall (k : int), 0 <= k < to_uint i => ( 0 <= to_uint output.[k] <= 15))
+).
+- if.
+    + auto => /> ; progress.
+        * rewrite to_uintD_small /#.
+        * smt(@W64).
+        * apply shr_ge0.
+        * split ; [ smt(@W64) | move => ? ; admit ].
+        * apply shr_lt_15.
+        * split ; first by smt(@W64). move => ? ; admit.
+        * pose t :=  (SHR_32 (zeroextu32 input{hr}.[to_uint in_0{hr}]) (truncateu8 ((of_int 4))%W64)).`6 `&` (of_int 15)%W32. rewrite get_setE. split ; [ smt() | move => ? ; smt ].
+          case (k = to_uint i{hr}). move => ?. apply shr_ge0. split ; admit. (* add invariant sobre in *)
+          move => ?. admit.
+        * rewrite get_setE. 
+          split ; [ smt() | move => ? ; admit ]. case (k = to_uint i{hr}). move => ?. apply shr_lt_15. split; by admit. admit.
+    + auto => />. progress.
+        * rewrite to_uintD_small /#. 
+        * smt(@W64).
+        * admit. (* add invariant sobre bits *)
+        * admit.   
+        * admit.
+        * admit.
+- auto => /> ; progress.
+    + smt.
+    + smt.
+    + smt.
+    + smt.
 qed.
 
-
-lemma shr_base_w (input : W8.t Array32.t) (output : W32.t Array67.t) (base_w : int list) (in_0 : W64.t) (k : int) (out : W64.t):
-to_uint
-  output.[to_uint out <-
-    (SHR_32 (zeroextu32 input.[to_uint in_0])
-       (truncateu8 ((of_int 4))%W64)).`6 `&`
-    (of_int 15)%W32].[k] =
-nth witness
-  (put base_w (to_uint out)
-     (to_uint
-        ((input.[to_uint in_0] `>>` (of_int 4)%W8) `&`
-         (of_int 15)%W8))) k.
-proof.
-admit.
-qed.
-
-lemma shr_base_w_2 (input : W8.t Array32.t) (output : W32.t Array67.t) (base_w : int list) (total : W8.t) (k : int) (bits out : W64.t):
-to_uint
-  output.[to_uint out <-
-    (SHR_32 (zeroextu32 total) (truncateu8 (bits - (of_int 4)%W64))).`6 `&`
-    (of_int 15)%W32].[k] =
-nth witness
-  (put base_w (to_uint out)
-     (to_uint
-        ((total `>>` (of_int (to_uint bits - 4))%W8) `&`
-         (of_int 15)%W8))) k.
-proof.
-admit.
-qed.
-
-
-lemma base_w_correctness_67_32 (_out : W32.t Array67.t, _in_ : W8.t Array32.t) :
+lemma base_w_spec_post :
     w = XMSS_WOTS_W =>
-    floor (log2 w%r) = XMSS_WOTS_LOG_W => 
-    equiv[M(Syscall).__base_w_67_32 ~ BaseW.base_w :
-      arg{1} = (_out, _in_) /\
-      arg{2} = (to_list _in_, 67) ==>
-        res{2} = map W32.to_uint (to_list res{1})].
+    hoare [BaseW.base_w : true ==> 
+    forall (k : int), 0 <= k <= size(res) => 0 <= nth witness res k <= w - 1].
 proof.
-rewrite /XMSS_WOTS_W /XMSS_WOTS_LOG_W.
-move => w_val logw.
+rewrite /XMSS_WOTS_W.
+move => w_val.
 proc.
-auto => /> *.
 while (
-  outlen{2} = 67 /\
-  0 <= to_uint consumed{1} <= 67 /\
-  consumed{2} = to_uint consumed{1} /\
-  X{2} = to_list input{1} /\
-  to_uint bits{1} = bits{2} /\
-  ={total} /\
-  0 <= _in{2} <= 67 /\
-  out{2} = to_uint out{1} /\
-  W64.zero \ule in_0{1} /\ in_0{1} \ule W64.of_int 67 /\
-  _in{2} = to_uint in_0{1} /\
-  forall (k : int), (0 <= k < out{2}) => to_uint (output{1}.[k]) = nth witness base_w{2} k
-).
-(* First subgoal of while *)
-if.
-(* First subgoal of if *)
-auto => /> *. smt.
-(* 2nd+3rd subgoals of if *)
-auto => /> *.
-do split.
-    - smt(@W64).
-    - smt(@W64).
-    - smt(plus_one).
-    - rewrite logw //.
-    - smt(@W64).
-    - smt.
-    - smt(plus_one).
-    - smt(@W64).
-    - smt.
-    - smt(plus_one).
-    - auto => /> *. rewrite logw. rewrite w_val //=. smt(shr_base_w).
-    - smt(@W64).
-    - smt.
-    - auto => /> *. do split.
-        - smt(@W64).
-        - smt(@W64).
-        - smt.
-        - rewrite logw. smt.       
-        - smt(plus_one). 
-        - auto => /> *. rewrite logw. rewrite w_val //=. smt(shr_base_w_2).
-        - smt(@W64).
-        - smt.
-(* Last subgoal of while *)
-auto => /> *. 
-do split.
-    - smt().
-    - auto => /> *. smt. 
-qed.
-
-(*
-expand seed :
-CORRECTNESS : Auxiliary lemmas with admit
-TERMINATION : NOT DONE
-*)
-
-lemma e0 (a : int) (b : W64.t):
-    a - to_uint b <= 0 => ! (b \ult W64.of_int a).
-proof.
-admit.
-qed.
-
-lemma expand_seed_correctness (outseeds : W8.t Array2144.t, inseed : W8.t Array32.t,
-                               pub_seed : W8.t Array32.t, addr : W32.t Array8.t) :
-    len = XMSS_WOTS_LEN =>
-    equiv [Mp(Syscall).__expand_seed ~ WOTS.pseudorandom_genSK :
-    arg{1} = (outseeds, inseed, pub_seed, addr) /\
-      arg{2} = (to_list inseed, to_list pub_seed, addr) ==> 
-        to_list res{1}.`1 = flatten res{2}].
-proof.
-rewrite /XMSS_WOTS_LEN.
-move => wots_len.
-proc.
-inline*.
-auto => />*.
-while (
-  len{2} = 67 /\
-  ={i}
-).
-admit.
-admit.
-qed.
-
-
-lemma expand_seed_ll : islossless Mp(Syscall).__expand_seed_.
-proof.
-proc ; inline => //=.
-islossless.
-while (true) (67 - i) => //= ; last by skip => /#. 
-auto => /> *.
-islossless ; first by smt().
-while (true) (8 - i1) ; last by skip ; auto => /> /#.
-auto => /> /#.
-while (true) (inlen - (to_uint i0)) => //=; last by skip => /> * ; smt(e0).
-auto => /> *. smt.
-qed.
-
-(* gen chain *)
-
-lemma b (i : W64.t) (t : int) : ! (i \ult (W64.of_int t)) <=> W64.of_int t \ule i by split ; by smt.
-lemma c (i : W64.t) : 64 - to_uint i <= 0 <=> (W64.of_int 64) \ule i by smt.
-
-lemma gen_chain_ll : islossless Mp(Syscall).__gen_chain.
-proof.
-proc.
-islossless.
-(* First *)
-while (cond = i \ult t /\ i \ult W32.of_int 16) (to_uint (t - i)).
-auto => />. 
-move => &h H cond.
-move : H => [#] a b c d e.
-split.
-admit.
-admit.
-admit.
-skip => /> *. split. admit.
-auto => /> *. admit.
-(* Last *)
-while (true) ((to_uint inlen) - (to_uint i)).
-auto => /> *.
-smt(@W64).
-skip => /> /#.
-qed.
-
-lemma gen_chain_inplace_ll : islossless Mp(Syscall).__gen_chain_inplace.
-proof.
-proc.
-islossless.
-while (cond = i \ult t /\ i \ult W32.of_int 16 /\ t = start + steps) (to_uint (t - i)). (* i < (start+steps) && i < XMSS_WOTS_W  *)
-auto => /> *.
-admit.
-admit.
-skip.
-auto => /> &h *.
-split.
-admit.
-auto => /> i0 H.
-pose x := start{h} + steps{h}.
-move => ?. admit. (* smt f0 should work but doesnt *)
-qed.
-
-(* checksum 
-CORRECTNESS : DONE
-TERMINATION : DONE
-*)
-lemma wots_checksum_correctness (msg : W32.t Array67.t) :
-    len1 = XMSS_WOTS_LEN1 => 
-    w = XMSS_WOTS_W =>
-    equiv [Mp(Syscall).__csum ~ WOTS.checksum :
-      arg{1} = msg /\ arg{2} = map W32.to_uint (to_list msg) ==> to_uint res{1} = to_uint res{2}].
-proof.
-rewrite /XMSS_WOTS_LEN_1 /XMSS_WOTS_W ; move => ? ?.
-proc => /=.
-while (
-  i{2} = to_uint i{1} /\
-  m{2} = map W32.to_uint (to_list msg_base_w{1}) /\
-  0 <= i{2} <= len1
-).
-auto => /> *.
-do split; 1,2,3,4,5: by smt.
-auto => /> *.
-split; 1: by smt().
-auto => /> *. smt.
-qed.
-
-lemma csum_ll : islossless Mp(Syscall).__csum.
-proof.
-proc.
-islossless.
-while (true) (64 - to_uint i).
-auto => /> &h i_lt64.
-smt. (* smt(@W64 @Int) fails *)
-auto => /> i *.  
-rewrite b.
-smt(c).
-qed.
-
-lemma checksum_ll : islossless Mp(Syscall).__wots_checksum.
-proof.
-proc.
-islossless.
-while (true) (to_uint (outlen - consumed)) ; last by skip => /> * ; smt(f0). auto => /> * ; smt(f2).
-while (true) (i - aux). auto => /#. skip => /> /#.
-while (true) (to_uint ((W64.of_int 64) - i)) ; last by skip => /> ; smt(f0). auto => /> * ; smt(f2).
-qed.
-
-(* 
-pkgen 
-TERMINATION : One subgoal with adimt. I want to apply the lemma gen_chain_inplace_ll
-CORRECTNESS :
-*)
-
-
-lemma wots_pkgen_ll : islossless Mp(Syscall).__wots_pkgen.
-proof.
-proc.
-islossless.
-- while (true) (67 - i) ; last by skip => /> /#. auto => /> *. admit. (* How do apply trhe lemma gen_chain_inplace_ll here *)
-- while (true) (67 - i) ; last by skip => /> /#. auto => /> *. islossless ; first by smt(). while (true) (8 - i) ; last by skip => /> /#. auto => /> *. islossless => /#.
-- while (true) (to_uint ((W64.of_int inlen) - i)) ; last by skip => /> * ;  smt(f0). auto => /> * ; smt(f2).
-qed.
-
-(*
-sign 
-TERMINATION : DONE
-CORRECTNESS : 
-*)
-lemma wots_sign_ll : islossless Mp(Syscall).__wots_sign.
-proof.
-proc.
-islossless.
-- while (true) (67 - i) ; last by skip => /> /#. auto => /> *. admit. (* How do I apply the lemma gen_chain_inplace_ll here? *)
-- while (true) (67 - i) ; last by skip => /> /#. auto => /> *. 
-  islossless; first by auto => /> /#. while (true) (8 - i); last by skip => /> /#. auto => /> *. islossless. auto => /> /#.
-- while (true) (to_uint ((W64.of_int inlen) - i)) ; last by skip => /> * ; smt(f0). auto => /> *. smt(f2).
-- while (true) (to_uint (outlen - consumed)); last by skip => /> ; smt(f0). auto => /> *. smt(f2).
-- while (true) (i - aux). auto => /#. skip => /> * ; smt(f1).
-- while (true) (to_uint ((W64.of_int 64) - i)); last by skip => /> * ; smt(f0). auto => /> *. smt(f2).
-- while (true) (to_uint (outlen - consumed)); last by skip => /> * ; smt(f0). auto => /> *. smt(f2).
-qed.
-
-(* 
-pk from sig 
-TERMINATION : One subgoal with admit
-CORRECTNESS :
-*)
-
-lemma wots_pk_from_sig_ll : islossless Mp(Syscall).__wots_pk_from_sig.
-proof.
-proc.
-islossless.
-- while (true) (67 - i) ; last by skip => /> /#. auto => /> *. islossless ; first by smt().
-   - admit. (* cond *)
-   - while (true) (to_uint (inlen - i)); last by skip => /> * ; smt(f0). auto => /> *. smt.
-- while (true) (to_uint (outlen - consumed)) ; last by skip => /> * ; smt(f0). auto => /> *. smt(f2).
-- while (true) (i - aux) ; last by skip => /> /#. auto => /> /#.
-- while (true) (to_uint ((W64.of_int 64) - i)) ; last by skip => /> * ; smt(f0). auto => /> ; smt(f2).
-- while (true) (to_uint (outlen - consumed)) ; last by skip => /> * ; smt(f0). auto => /> *; smt(f2).
+true
+) ; by admit.
 qed.
