proof/spec/XMSS_MT_PRF.ec
@@ -1,0 +1,518 @@
+pragma Goals : printall.
+
+require import AllCore List RealExp IntDiv.
+require (*--*) Subtype. 
+
+from Jasmin require import JModel.
+
+require import Params Notation Parameters Address Primitives Wots.
+
+import NBytes.
+import Array8.
+
+require import XMSS.
+
+clone import Subtype as Bitmask with 
+   type T = byte list,
+   op P = fun l => size l = 2 * n
+   rename "T" as "bitmask"
+   proof inhabited by (exists (nseq (2*n) W8.zero);smt(size_nseq ge0_n))
+   proof *.
+
+clone import Subtype as Three_NBytes with 
+   type T = byte list,
+   op P = fun l => size l = 3 * n
+   rename "T" as "three_n_bytes"
+   proof inhabited by (exists (nseq (3*n) W8.zero);smt(size_nseq ge0_n))
+   proof *.
+
+clone import Subtype as OTSKeys with 
+   type T = wots_sk list,
+   op P = fun l => size l = 2^h
+   rename "T" as "wots_ots_keys".
+clone import Subtype as AuthPath with
+  type T = nbytes list,
+  op P = fun l => size l = len
+  rename "T" as "auth_path"
+  proof inhabited by (exists (nseq len (nseq n W8.zero));smt(size_nseq ge0_len))
+  proof *.
+
+op d : { int | 1 <= d } as ge1_d. (* d layers of trees, each having height h/d  *)
+op h : { int | 0 <= h /\ h %% d = 0} as h_vals. (* hyper-tree of total height h, where h is a multiple of d *)
+
+(**********************************************************************************************)
+
+(* gets the n most significant bits *)
+op msb (x : byte list) (n : int) : byte list = take n x. 
+
+(* gets the n most significant bits of x *)
+(* n is at most 32 *)
+op msb_w32 (x : W32.t) (n : int) : bool list = take n (w2bits x).
+
+(* Returns the n most significant bits of x as a W32.t *)
+op msb_w32_int (x : W32.t) (n : int) : W32.t = 
+  let bits : bool list = take n (w2bits x) in
+  (W32.bits2w bits).
+
+op lsb_w32_int (x : W32.t) (n : int) : W32.t =
+   let bits : bool list =  w2bits x in
+   let lsbits : bool list =  drop ((size bits) - n) bits in
+   W32.bits2w lsbits.
+
+(**********************************************************************************************)
+
+op H : nbytes -> bitmask -> nbytes.
+op H_msg : three_n_bytes -> byte list -> nbytes.
+op _prf_ : nbytes -> byte list -> nbytes.
+op impl_oid : W32.t.
+
+(**********************************************************************************************)
+
+type xmss_mt_sk = { idx : W32.t ;
+                    sk_seed : nbytes ; (* secret *)
+                    sk_prf : nbytes ;
+                    pub_seed_sk : nbytes ; (* public *)
+                    sk_root : nbytes }.
+
+type xmss_mt_pk = { pk_oid : W32.t ;
+                    pk_root : nbytes ;
+                    pk_pub_seed : nbytes }.
+
+type msg_t = byte list.
+
+type sig_t = { sig_idx : W32.t;
+               r : nbytes;
+               wots_sig : wots_signature;
+               authentication_path : auth_path }.
+
+type xmss_mt_keypair = xmss_mt_sk * xmss_mt_pk.
+
+(**********************************************************************************************)
+
+(* 4.1.4 Randomized tree hashing *)
+op rand_hash (_left _right : nbytes, _seed : seed, address : adrs) : nbytes = 
+  let address : adrs = set_key_and_mask address 0 in
+  let key : nbytes = PRF _seed address in
+  let address : adrs = set_key_and_mask address 1 in
+  let bitmask_0 : nbytes = PRF _seed address in
+  let address : adrs = set_key_and_mask address 2 in
+  let bitmask_1 : nbytes = PRF _seed address in
+  let hash_in : nbytes = (nbytexor _left bitmask_0) ++ (nbytexor _right bitmask_1) in
+  H key hash_in.
+
+(**********************************************************************************************)
+
+(* 4.1.5 L-Trees *)
+module LTree = {
+  proc ltree (pk : wots_pk, address : adrs, _seed : seed) : nbytes = {
+    var pk_i : nbytes;
+    var tmp : nbytes;
+    var i : int <- witness;
+    var _len : int <- len;
+
+    address <- set_tree_height address 0;
+
+    while (1 < _len) { (* Same as _len > 1 *)
+      i <- 0;
+      while (i < floor (len%r / 2%r)) {
+        address <- set_tree_index address i;
+        pk_i <- nth witness pk (2*i);
+        tmp <- nth witness pk (2*i + 1);
+        pk_i <- rand_hash pk_i tmp _seed address;
+        pk <- put pk i pk_i;
+      }
+
+      if (_len %% 2 = 1) {
+        pk_i <- nth witness pk (_len - 1);
+        pk <- put pk (floor (len%r / 2%r)) pk_i;
+      }
+
+      _len <- ceil (len%r / 2%r);
+      i <- i + 1;
+    }
+
+    pk_i <- nth witness pk 0;
+
+    return pk_i;
+  }
+}. 
+
+
+lemma neg_lt (x y : int) : ! (x < y) <=> y <= x by smt().
+
+
+lemma ltree_ll : islossless LTree.ltree.
+proof.
+proc.
+sp ; wp.
+while (1 <= _len <= len) (_len - 1) ; auto => />.
+- while (0 <= i <= floor (len%r / 2%r)) (floor (len%r / 2%r) - i) ; auto => />.
+  + progress. rewrite neg_lt. admit.
+  + progress; 1,2,3,4,5: by admit.
+- split ;  [ smt(g0_len) | move => * ; rewrite neg_lt /# ].
+qed.
+
+(**********************************************************************************************)
+
+(* Stack operations *)
+abbrev push (x : 'a list) (a : 'a) : 'a list = rcons x a. 
+
+op remove_last (x : 'a list) : 'a list = 
+with x = [] => []
+with x = h::t => if t = [] then [] else remove_last t.
+
+abbrev pop (x : 'a list) : 'a list * 'a = 
+    let last_elem : 'a = last witness x in
+    let new_list = remove_last x in
+    (new_list, last_elem).
+
+(* It is REQUIRED that s % 2^t = 0, i.e., that the leaf at index s is a leftmost leaf of a sub-tree of height t. *)
+pred leftmost_leaf (s t : int)  = s %% 2^t = 0.
+
+pred treehash_p (s t : int) = s %% (1 `<<` t) <> 0.
+
+
+(* NOTE: In the implementation, treehash (in xmss_core.c) computes both the authentication 
+         path and the resulting root node *)
+module TreeHash = {
+  (* Computes the root *)
+  proc treehash(sk : xmss_mt_sk, s t : int, address : adrs) : nbytes = {
+  var node : nbytes;
+  var stack : nbytes list;
+  var top_node : nbytes;
+  var pub_seed : seed <- sk.`pub_seed_sk;
+  var sk_seed : seed <- sk.`sk_seed;
+  var pk : wots_pk;
+  var i : int <- 0;
+  var tree_index, tree_height: int;
+  var heights : int list;
+  var tmp : int;
+  var offset : int <- 0;
+    
+    while (i < 2^t) {
+      (* ----------- not in the RFC ----------- *)
+      offset <- offset + 1;
+      heights <- put heights (offset - 1) 0; 
+      (* -------------------------------------- *)
+
+      address <- set_type address 0;
+      address <- set_ots_addr address (s + 1);
+
+      (* Generate the public key from the secret seed *)
+      pk <@ WOTS.pkGen(sk_seed, pub_seed, address);
+
+      address <- set_type address 1;
+      address <- set_tree_addr address (s + 1);
+
+      node <@ LTree.ltree(pk, address, pub_seed); 
+
+      address <- set_type address 2;
+      address <- set_tree_height address 0;
+      address <- set_tree_index address (i + 1);
+      
+      top_node <- last witness stack;
+
+      (* While the top-most nodes are of equal height *)
+      (* offset >= 2 <=> 2 <= offset *)
+      
+      while (2 <= offset /\ ((nth witness heights (offset - 1)) = (nth witness heights (offset - 2)))) {
+        tree_index <- get_tree_index address;
+        address <- set_tree_index address (ceil((tree_index - 1)%r / 2%r));
+        (stack, top_node) <- pop stack;
+
+        node <- rand_hash top_node node pub_seed address;
+        
+        (* ----------- not in the RFC ----------- *)
+        offset <- offset - 1;
+        tmp <- nth witness heights (offset - 1);
+        heights <- put heights (offset - 1) (t + 1);
+        (* -------------------------------------- *)
+
+        tree_height <- get_tree_height address;
+        address <- set_tree_height address (tree_height + 1); (* Move to the next tree *)
+      }
+
+      stack <- push stack node;
+      i <- i + 1;
+    }
+    
+  return node;
+  }
+}.
+
+lemma treehash_ll : islossless TreeHash.treehash.
+proof.
+proc.
+sp ; wp.
+while (true) (2^t - i) ; auto => /> ; last by progress ; rewrite neg_lt /#.
+sp ; wp. 
+admit.
+qed.
+
+module TreeSig = {
+  proc buildAuthPath(sk : xmss_mt_sk, idx : W32.t, address : adrs) : auth_path = {
+    var authentication_path : auth_path;
+    
+    var j : int <- 0;
+    var k : int;
+    var t : nbytes <- witness;
+
+    while (j < h) {
+      k <- floor((W32.to_uint idx)%r / (2^j)%r);
+      t <@ TreeHash.treehash(sk, k * (2^j), j, address);
+      authentication_path <- put authentication_path j t;
+      j <- j+1;
+    }
+
+    return authentication_path;
+  }
+
+  proc treesig(M : nbytes, sk : xmss_mt_sk, idx : W32.t, address : adrs) : wots_signature * auth_path  = {
+    var auth : auth_path;
+    var sig_ots : wots_signature;
+    var ots_sk : wots_sk;
+    var seed : nbytes;
+    
+    auth <@ buildAuthPath (sk, idx, address);
+    address <- set_type address 0;
+    address <- set_ots_addr address (W32.to_uint idx);
+
+    sig_ots <@ WOTS.sign_seed(M, sk.`sk_seed, sk.`pub_seed_sk, address);
+    
+    return (sig_ots, auth);
+  }
+}.
+
+lemma buildAuthPath_ll : islossless TreeSig.buildAuthPath.
+proof.
+proc.
+while (0 <= j <= h) (h - j) ; auto => />.
+  - call treehash_ll ; auto => /> /#. 
+  - split ; smt(h_vals). 
+qed.
+
+lemma treesig_ll : islossless TreeSig.treesig.
+proof.
+proc.
+call wots_sign_seed_ll.
+auto => /> ; call buildAuthPath_ll.
+by skip.
+qed.
+
+ (**********************************************************************************************)
+
+op append_sig (sig : sig_mt) (sig_tmp : reduced_sig) : sig_mt =    
+    let new_sigs: reduced_sig list = sig.`reduced_sig_mt  ++  [sig_tmp] in
+    {| sig with  reduced_sig_mt=new_sigs|}.
+
+
+module XMSS_MT_PRF = {
+   proc kg() : xmss_mt_keypair = {
+      var pk : xmss_mt_pk <- witness;
+      var sk : xmss_mt_sk <- witness;
+
+      var idx_MT : W32.t <- W32.zero;
+      var sk_seed, sk_prf, pub_seed, root : nbytes;
+
+      var address : adrs <- zero_address;
+      
+      sk_seed <$ DList.dlist W8.dword n;
+      sk_prf <$ DList.dlist W8.dword n;
+      pub_seed <$ DList.dlist W8.dword n;
+
+      root <@ TreeHash.treehash(sk, 0, h, address);
+
+      sk <- {| idx=idx_MT;
+               sk_seed=sk_seed;
+               sk_prf=sk_prf;
+               pub_seed_sk=pub_seed;
+               sk_root=root;
+             |};
+
+      pk <- {| pk_oid=impl_oid; pk_root=root; pk_pub_seed=pub_seed |};
+
+      return (sk, pk);
+   }
+
+   proc rootFromSig(idx_sig : W32.t, sig_ots : wots_signature, auth : auth_path, M : nbytes, 
+                   _seed : seed, address : adrs) : nbytes = {
+    var pk_ots : wots_pk;
+    var k : int <- 0;
+    var nodes0, nodes1 : nbytes;
+    var index : int;
+    var auth_k : nbytes;
+    
+    address <- set_type address 0;
+    address <- set_ots_addr address (W32.to_uint idx_sig);
+
+    pk_ots <@ WOTS.pkFromSig(M, sig_ots, _seed, address);
+
+    address <- set_type address 1;
+    address <- set_ltree_addr address (W32.to_uint idx_sig);
+
+    nodes0 <@ LTree.ltree(pk_ots, address, _seed);
+
+    address <- set_type address 2;
+    address <- set_tree_index address (W32.to_uint idx_sig);
+
+    while (k < h) {
+      address <- set_tree_height address k;
+
+      if (floor ((W32.to_uint idx_sig)%r / (2^k)%r) %% 2 = 0) {
+        index <- get_tree_index address;
+        address <- set_tree_index address (index %/ 2);
+
+        auth_k <- nth witness auth k;
+        nodes1 <- rand_hash nodes0 auth_k _seed address;
+      } else {
+        index <- get_tree_index address;
+        address <- set_tree_index address ((index - 1) %/ 2);
+
+        auth_k <- nth witness auth k;
+        nodes1 <- rand_hash auth_k nodes0 _seed address;
+      }
+
+      nodes0 <- nodes1;
+      k <- k+1;
+    }
+
+    return nodes0;
+  }
+
+
+
+   proc sign(sk : xmss_mt_sk, m : msg_t) : sig_mt * xmss_mt_sk = {
+      var sig : sig_mt;
+      var idx : W32.t <-sk.`idx;
+      var idx_new : W32.t;
+      var idx_bytes : byte list;
+      var idx_nbytes : nbytes;
+      var idx_tree : W32.t;
+      var idx_leaf : W32.t;
+      var _R : nbytes;
+      var _M' : nbytes;
+      var address : adrs <- zero_address;
+      var root : nbytes <- sk.`sk_root;
+      var t : three_n_bytes;
+      var sk_prf : nbytes <- sk.`sk_prf;
+      var j : int;
+      var pub_seed : nbytes <- sk.`pub_seed_sk;
+      var sig_tmp : wots_signature;
+      var auth : auth_path;
+    
+
+      (* Update the key index *)
+      idx_new <- idx + W32.one;
+      sk <- {| sk with idx=idx_new |};
+
+      idx_bytes <- toByte idx 32;
+      _R <- _prf_ sk_prf idx_bytes;
+
+      idx_nbytes <- toByte idx n;
+      t <- _R ++ root ++ idx_nbytes;
+      _M' <- H_msg t m;
+
+      idx_tree <- msb_w32_int idx (h - (h %/ d));
+      idx_leaf <- msb_w32_int idx (h %/ d);
+
+      address <- set_layer_addr address 0;
+      address <- set_tree_addr address (W32.to_uint idx_tree);
+
+      (sig_tmp, auth) <@ TreeSig.treesig(_M', sk, idx_leaf, address);
+     
+      sig <- {| sig with reduced_sig_mt=[(sig_tmp, auth)] |};
+
+      j <- 1;
+      while (j < d) {
+      root <@ TreeHash.treehash(sk, 0, h %/ d, address);
+      idx_leaf <- lsb_w32_int idx_tree (h %/ d);
+      idx_tree <- msb_w32_int idx_tree (h - (j * (h %/ d)));
+      
+      address <- set_layer_addr address j;
+      address <- set_tree_addr address (W32.to_uint idx_tree);
+
+      (sig_tmp, auth) <@ TreeSig.treesig(root, sk, idx_leaf, address);
+      
+      sig <- append_sig sig (sig_tmp, auth);
+      
+      
+      j <- j+1;
+    }
+      
+
+      return (sig, sk);
+   }
+
+   proc verify(pk : xmss_mt_pk, m : msg_t, s : sig_mt) : bool = {
+     var is_valid : bool;
+     var idx : W32.t <- s.`sig_idx_mt;
+     var idx_bytes : nbytes <- toByte idx n;
+     var seed : nbytes <- pk.`pk_pub_seed;
+     var address : adrs <- zero_address;
+     var idx_leaf : W32.t <- lsb_w32_int idx (h %/ d);
+     var idx_tree : W32.t <- msb_w32_int idx (h - (h %/ d));
+     var _sig : reduced_sig;
+     var node, root, _R, _M': nbytes;
+     var t : three_n_bytes;
+     var j : int;
+
+      _sig <- nth witness s.`reduced_sig_mt 0;
+
+      _R <- s.`r_mt;
+     root <- pk.`pk_root;
+     t <- _R ++ root ++ idx_bytes;
+      _M' <- H_msg t m; 
+     
+     node <@ XMSS.rootFromSig(idx_leaf, _sig.`1, _sig.`2, _M', seed, address);
+
+     j <- 1;
+     while (j < d) {
+       idx_leaf <- lsb_w32_int idx_tree (h %/ d);
+       idx_tree <- msb_w32_int idx_tree (h - (h %/ d));
+
+       _sig <- nth witness s.`reduced_sig_mt j;
+      
+       address <- set_layer_addr address j;
+       address <- set_tree_addr address (W32.to_uint idx_tree);
+
+       node <@ XMSS.rootFromSig(idx_leaf, _sig.`1, _sig.`2, _M', seed, address);
+
+       j <- j + 1;
+     }
+
+    is_valid <- (node = root);
+
+
+
+     return is_valid;
+   }
+}.
+
+lemma xmss_mt_kg_ll : islossless XMSS_MT_PRF.kg.
+proof.
+proc.
+auto => /> ; call treehash_ll.
+auto => /> *. smt.
+qed.
+
+lemma root_from_sig_ll : islossless XMSS_MT_PRF.rootFromSig.
+proof.
+proc.
+while (0 <= k <= h) (h - k) ; auto => /> ; 1,2: by progress ; smt().
+call ltree_ll ; auto => />. 
+call wots_pkFromSig_ll ; auto => />.
+smt(h_vals).
+qed.
+
+lemma xmss_mt_sign_ll : islossless XMSS_MT_PRF.sign.
+proof.
+proc.
+while (0 <= j <= d) (d - j) ; auto => />.
+  - call treesig_ll ; auto => />. call treehash_ll. skip => /> /#.
+  - progress ; smt().
+  - call treesig_ll ; auto => /> ; smt(ge1_d).
+qed.
+
+axiom prf_keygen : equiv [XMSS_MT.kg ~ XMSS_MT_PRF.kg : true ==> true].
+
+
